::: {.content-hidden}
$
{{< include macros.tex >}}
$
:::




# Curvature and Torsion

We have seen how to describe curves and reparametrized them. Now we want to look at local properties of curves:

- How much does a curve twist?
- How much does a curve bend?

We will measure two quantities:

- **Curvature**: measures how much a curve $\g$ deviates from a straight line.
- **Torsion**: measures how much a curve $\g$ fails to lie on a plane.

For example a 2D spiral is curved, but still lies in a plane. Instead the Helix both deviates from a straight line and *pulls away* from any fixed plane. 



## Curvature 

We start with an informal discussion. Suppose $\g$ is a straight line
$$
\g(t) = \mathbf{a} + t \mathbf{v}
$$
with $\mathbf{a}, \mathbf{v} \in \R^3$. The tangent vector to $\g$ is constant
$$
\dot\g(t) =  \mathbf{v} \,.
$$
Whatever the definition of curvature will be, it has to hold that $\g$ has zero curvature in this case. If we further derive the tangent vector, we obtain
$$
\ddot\g(t) =  \zero \,.
$$
Thus $\ddot \g$ seems to be a good candidate for the definition of curvature of $\g$ at the point $\g(t)$.  


Suppose now that $\g$ is a curve in $\R^2$ with unit speed. We have proven that in this case
$$
\dot \g \cdot \ddot\g = 0 \,,
$$
that is, the vector $\ddot \g$ is orthogonal to the tangent $\dot \g$ at all times. Now let $\mathbf{n}(t)$ be the unit vector orthogonal to $\dot \g(t)$ at the point $\g(t)$. The amount that the curve $\g$ deviates from its tangent at $\g(t)$ after time $t_0$ is
$$
( \g(t + t_0) - \g(t) ) \cdot \mathbf{n}(t) \,,
$$ {#eq-curvature-heuristics}
as seen in the figure below.


![Amount that $\g$ deviates from tangent is $(\g(t+t_0)-\g(t)) \cdot \nn(t)$](/images/curvature.png){width=70%}


Equation (@eq-curvature-heuristics) is what we take as measure of curvature. Since 
$$
\dot \g(t) \cdot \ddot \g(t) = 0 \quad \mbox{ and } \quad   \dot \g(t) \cdot \mathbf{n}(t)= 0 \,,
$$
we conclude that $\ddot \g(t)$ is parallel to $\mathbf{n}(t)$. Since $\mathbf{n}(t)$ is a unit vector, there exists a scalar $\kappa(t)$ such that 
$$
\ddot \g(t)  = \kappa(t) \, \mathbf{n}(t) \,.
$$
Note that, since $\nn$ is unitary, we have
$$
\kappa(t) = \norm{ \ddot \g(t) }
$$


Now, approximate $\g$ at $t$ with its second order Taylor polynomial:
$$
\g(t+t_0) = \g(t) + \dot\g(t) t_0 + \frac{\ddot\g(t)}{2} t_0^2 + o(t_0)
$$
with the remainder $o(t_0)$ is such that 
$$
\lim_{t_0 \to 0} \ \frac{o(t_0)}{t_0^2} = 0 \,.
$$
Therefore, forgetting about the remainder, 
$$
\g(t+t_0) - \g(t) \approx \dot\g(t) t_0 + \frac{\ddot\g(t)}{2} t_0^2 \,.
$$
Multiplying by $\nn(t)$ we get
$$
(\g(t+t_0) - \g(t)) \cdot \nn(t) \approx \dot\g(t) \cdot \nn(t) t_0 + 
\frac{\ddot\g(t) \cdot \nn(t) }{2} t_0^2\,.
$$
Recalling that 
$$
\dot\g(t) \cdot \nn(t) = 0\,, \quad  \ddot\g(t) \cdot \nn(t) = \kappa(t) \,, 
$$
we then obtain
$$
(\g(t+t_0) - \g(t)) \cdot \nn(t) \approx 
\frac{1}{2} \, \kappa(t) \, t_0^2
$$


::: Important

The amount that $\g$ deviates from a straight line is proportional to 
$$
\kappa(t) = \norm{\ddot \g (t)}\,.
$$

:::

We take this as definition of curvature for a general unit speed curve in $\R^n.$


::: Definition 

Let $\g \ \colon (a,b) \to \R^n$ be a unit speed curve. The **curvature** of $\g$ at $\g(t)$ is
$$
\kappa^\g(t) := \norm{\ddot \g (t)} \,.
$$

:::



Note that $\kappa(t)$ is a function of time. Therefore the curvature of $\g$ can change from point to point.


We now define curvature for curves which are regular, but not necessarily unit speed.


::: Definition 

Let $\g \ \colon (a,b) \to \R^n$ be a regular. The **curvature** of $\g$ at $\g(t)$ is
$$
\kappa^\g(t) :=   \norm{\ddot{\tg} (\f(t))} \,, \quad \forall \, t \in (a,b)\,,
$$
where $\tg$ is a unit speed reparametrization of $\g$, with $\g = \tg \circ \f$.

:::


::: Remark

The above definition is well posed:

- Since $\g$ is regular, there exist a unit speed reparametrization $\tg$ of $\g$.
- If $\hat{\g}$ is another unit speed reaprametrization of $\g$, with $\g = \hat{\g} \circ \hat\f$, then
$$
\kappa^{\g} (t) =   \norm{\ddot{\hat\g} (\hat\f(t))} \,,
$$
showing that there is no ambiguity in the definition of $\kappa^\g$.

> Indeed, since $\tg$ and $\hat{\g}$ are both reparametrizations of $\g$, then 
$$
\g(t) = \tg(  \tilde{\f}(t)) \,, \quad 
\g(t) = \hat{\g} (\hat{\f}(t)  ) 
$$
for some diffeomorphisms $\tilde{\f}, \hat{\f}$. Hence 
$$
{\tg}(t) = \hat\g(\f(t))\,, \quad \f := \hat{\f} \circ (\tilde{\f})^{-1} \,,
$${#eq-well-posed-curvature-3}
where $\f$ is a diffeomorphism, since it is composition of diffeomorphisms. 
Differentiating (@eq-well-posed-curvature-3) we get
$$
\dot{\tg}(t) = \dot{\hat{\g}}(\f(t)) \dot\f(t) \,.
$${#eq-well-posed-curvature-2}
Taking the norms of the above, and recalling that $\tg$ and $\hat\g$ are unit speed, we get
$$
|\dot\f(t)| = 1 \,, \quad  \forall \, t \,. 
$${#eq-well-posed-curvature}
Since $\f$ is a diffeomorphism, we already know that $|\dot\f| \neq 0$. As $\dot\f$ is continuous, this means that the sign of $\dot\f$ is constant. Thus (@eq-well-posed-curvature) implies 
$$
\dot\f(t) \equiv 1 \quad \mbox{or} \quad
\dot\f(t) \equiv -1 \,.
$$
In both cases, we have
$$
\ddot \f \equiv 0 \,.
$$
Differentiating (@eq-well-posed-curvature-2) we then obtain
\begin{align}
\ddot{\tg}(t) & = \ddot{\hat{\g}}(\f(t)) \dot\f^2(t) + 
                         \dot{\hat{\g}}(\f(t)) \ddot\f (t) \\
                  & = \ddot{\hat{\g}}(\f(t)) \dot\f^2(t) \,.
\end{align}
Taking the norms and using again that $|\dot\f| \equiv 1$, we get  that 
$$
\norm{  \ddot{\tg}(t)} = \norm{ \ddot{\hat{\g}}(\f(t))} \,.
$$
Recalling that $\phi  = \hat\f \circ (\tilde{\f})^{-1}$ we get
$$
\norm{  \ddot{\tg}( \tilde{\f}(t))} = \norm{ \ddot{\hat{\g}}(\hat\f(t))} \,, \quad \forall \, t \in (a,b) \,.
$$
Therefore 
$$
\kappa^\g(t) =  \norm{  \ddot{\tg}( \tilde{\f}(t))} = \norm{ \ddot{\hat{\g}}(\hat\f(t))} \,.
$$

:::



::: Remark 
### Methods for computing curvature

In summary, the curvature of a regular curve 
$$
\g \ \colon (a,b) \to \R^n
$$ 
is defined via unit speed reparametrizations of $\g$. To compute $\kappa$ we do the following: 

- We find a unit speed reparametrization $\tg$ of the regular curve $\g$
- This can be done by computing $s$ the arc-length of $\g$, and then defining 
$$
\tg:= \g \circ \psi \,, \quad \psi:=s^{-1} 
$$
- Then we compute 
$$
\kappa^{\tg}(t) = \norm{\ddot{\tg}}(t)
$$
- We obtain the curvature of $\g$ by
$$
\kappa^\g (t)= \kappa^{\tg} (t) 
$$

When $\g$ is regular and has values in $\R^3$, there is a way to compute $\kappa$ without reparametrizing. To do this, we will need the notion of **cross product**, or **vector product**. We will see this in the following sections.
:::


![Procedure for computing curvature $\kappa$](/images/curvature_shortcut.png){width=70%}



We conclude with an example where we compute $\kappa$ using reparametrizations.


::: Example

Consider the circle of radius $R>0$:
$$
\g(t) = (R\cos(t),R\sin(t)) \,, \quad t \in [0,2\pi] \,.
$$
To compute the curvature of $\g$ we need to find a unit speed reparametrization. We have shown that:
$$
\g \, \mbox{ regular } \,\,\, \implies \,\,\, \f = s^{-1} \, \mbox{ unit speed reparametrization}
$$
where $s$ is the arc length of $\g$:
$$
s(t):= \int_{t_0}^t \norm{\dot \g(\tau)} \, d\tau  \,.
$$
In our case 
$$
\dot \g(t) = (-R\sin(t), R\cos(t))  \quad \implies \quad 
\norm{\dot \g(t)} = R  
$$
and so $\g$ is regular. The arc length starting at $t_0 = 0$ is
$$
s(t) = \int_{0}^t R d \tau = t R \,.
$$
The inverse of $s$ is
$$
\f(t) := s^{-1} (t) = \frac{t}{R} \,.
$$
Therefore a unit speed reparametrization of $\g$ is 
$$
\tg :=\g \circ \f 
$$
which reads
$$
\tg(t) :=  \left( R \cos \left( \frac{t}{R} \right) , R \sin \left( \frac{t}{R} \right)\right) \,.
$$
We have
\begin{align}
\dot{\tg} (t) & =  \left( - \sin \left( \frac{t}{R} \right) ,  \cos \left( \frac{t}{R} \right)\right) \\
\ddot{\tg} (t) & =  \left( -\frac{1}{R} \cos \left( \frac{t}{R} \right) ,  - \frac{1}{R} \sin \left( \frac{t}{R} \right)\right)
\end{align}
Therefore the curvature of $\g$ is
$$
\kappa(t) = \norm{ \ddot{\tg} (t) } = \frac{1}{R} \,.
$$
In this case $\kappa(t)$ is constant. The curvature also tells us that the smaller the circle, the higher the curvature. For a large circle, like the Earth, the curvature is barely noticeable. 
:::








## Vector product in $\R^3$


The discussion in this section follows [@do-carmo]. We start by defining **orientation** for a vector space.


::: Definition
### Same orientation

Consider two ordered basis of $\R^3$
$$
B = (\bb_1,\bb_2,\bb_3) \,, \quad \tilde{B} = (\widetilde{\bb}_1,\widetilde{\bb}_2,\widetilde{\bb}_3) \,.
$$
We say that $B$ and $\widetilde{B}$ have the same orientation if the matrix of change of basis has positive determinant.

:::

When two basis $B$ and $\widetilde{B}$ have the same orientation, we write
$$
\bb \sim \widetilde{\bb} \,.
$$
The above is clearly an equivalence relation on the set of ordered basis. Therefore the set of ordered basis of $\R^3$ can be decomposed into equivalence classes.
Since the determinant of the matrix of change of basis can only be positive or negative, there are only two equivalence classes.


::: Definition 
### Orientation

The two equivalence classes determined by $\sim$ on the set of ordered basis are called **orientations**. 

:::



::: Definition 
### Positive orientation

Consider the standard basis of $\R^3$ 
$$
E = (\ee_1,\ee_2,\ee_3)
$$
where we set
$$
\ee_1 = (1,0,0)\,, \quad \ee_2 = (0,1,0) \,, \quad \ee_3 = (0,0,1) \,.
$$
Then:

- The orientation corresponding to $E$ is called **positive orientation** of $\R^3$.
- The orientation corresponding to the other equivalence class is called **negative orientation** of $\R^3$.


For a basis $B$ of $\R^3$ we say that:

- $B$ is a **positive basis** if it belongs to the class of $e$.
- $B$ is a **negative basis** if it does not belong to the class of $e$.
:::



::: Example

Since we are dealing with ordered basis, the order in which vectors appear is fundamental. For example, we defined the equivalence class of
$$
E = (\ee_1,\ee_2,\ee_3) \,,
$$
to be the positive orientation of $\R^3$. In particular $e$ is a positive basis.  
Consider instead
$$
\widetilde{E} = (\ee_2,\ee_1,\ee_3) \,.
$$
The matrix of change of variables between $\widetilde{E}$ and $E$ is 
$$
(\ee_2 | \ee_1 | \ee_3 ) = \left(
\begin{array}{ccc}
0 & 1 & 0 \\ 
1 & 0 & 0 \\
0 & 0 & 1 \\
\end{array}
\right)
$$
and the latter has negative determinant. Thus $\widetilde{E}$ does not belong to the class of $E$, and is therefore a negative basis. 
:::


We are now ready to define the vector product in $\R^3$.


::: Definition
### Vector product in $\R^3$   

Let $\uu,\vv \in \R^3$. The vector product of $\uu$ and $\vv$ is the unique vector 
$$
\uu \times \vv \in \R^3
$$
which satisfies the property:
$$
(\uu \times \vv) \cdot \ww = 
\left|
\begin{array}{ccc}
u_1 & u_2 & u_3 \\
v_1 & v_2 & v_3 \\
w_1 & w_2 & w_3 \\
\end{array}
\right| \,, \quad \forall \, \ww \in \R^3 \,.
$${#eq-def-vector-product}
Here $|a_{ij}|$ denotes the determinant of the matrix $(a_{ij})$, and 
$$
\uu= \sum_{i=1}^3 u_i \ee_i \,, \quad
\vv= \sum_{i=1}^3 v_i \ee_i \,, \quad
\ww= \sum_{i=1}^3 w_i \ee_i \,,
$$
with $(\ee_1,\ee_2,\ee_3)$ standard basis of $\R^3$.
:::


The following proposition gives an explicit formula for computing $\uu \times \vv$.


::: Proposition

Let $\uu,\vv \in \R^3$. Then
$$
\uu \times \vv = 
\left|
\begin{array}{cc}
u_2 & u_3  \\
v_2 & v_3 
\end{array}
\right| \ee_1 -
\left|
\begin{array}{cc}
u_1 & u_3  \\
v_1 & v_3 
\end{array}
\right| \ee_2 +
\left|
\begin{array}{cc}
u_1 & u_2  \\
v_1 & v_2 
\end{array}
\right| \ee_3  \,. 
$$ {#eq-formula-cross-product}
:::


::: Proof
Denote by $(\uu \times \vv)_i$ the $i$-th component of $\uu \times \vv$ with respect to the standard basis, that is,
$$
\uu \times \vv = \sum_{i=1}^3  (\uu \times \vv)_i \, \ee_i \,.
$$
We can use (@eq-def-vector-product) with $\ww = \ee_1$ to obtain 
$$
(\uu \times \vv) \cdot \ee_1  = 
\left|
\begin{array}{ccc}
u_1 & u_2 & u_3 \\
v_1 & v_2 & v_3 \\
 1  & 0   &   0 \\
\end{array}
\right| =
\left|
\begin{array}{cc}
u_2 & u_3  \\
v_2 & v_3 
\end{array}
\right|
$$
where we used the Laplace expansion for computing the determinant of the $3 \times 3$ matrix. As the standard basis is orthonormal, by bilinearity of the scalar product we get
$$
(\uu \times \vv) \cdot \ee_1 = \sum_{i=1}^3  (\uu \times \vv)_i \, \ee_i \cdot \ee_1 = (\uu \times \vv)_i \,.
$$
Therefore we have shown
$$
(\uu \times \vv)_1 = \left|
\begin{array}{cc}
u_2 & u_3  \\
v_2 & v_3 
\end{array}
\right| \,.
$$
Similarly we obtain
$$
(\uu \times \vv)_2  = \left|
\begin{array}{ccc}
u_1 & u_2 & u_3 \\
v_1 & v_2 & v_3 \\
 0  & 1   &   0 \\
\end{array}
\right| = -
\left|
\begin{array}{cc}
u_1 & u_3  \\
v_1 & v_3 
\end{array}
\right|
$$
and 
$$
(\uu \times \vv)_3  = \left|
\begin{array}{ccc}
u_1 & u_2 & u_3 \\
v_1 & v_2 & v_3 \\
 0  & 0   &   1 \\
\end{array}
\right| = 
\left|
\begin{array}{cc}
u_1 & u_2  \\
v_1 & v_2 
\end{array}
\right| \,,
$$
from which we conclude.
:::





::: {.Proposition #proposition-vector-product}

The vector product in $\R^3$ satisfies the following properties: For all $\uu, \vv \in \R^3$ 

1. $\uu \times \vv = - \vv \times \uu$
2. $\uu \times \vv = \zero$ if and only if $\uu$ and $\vv$ are linearly dependent
3. $(\uu \times \vv) \cdot \uu = 0$, $(\uu \times \vv) \cdot \vv = 0$
4. Moreover for all $\ww \in \R^3$, $a,b \in \R$
$$
(a\uu + b\ww) \times \vv = a \uu \times \vv + b\ww \times \ww 
$$

:::

The proof, which is based on the properties of determinants, is omitted.


::: Remark
### Geometric interpretation of vector product

Let $\uu, \vv \in \R^3$ be linearly independent. We make some observations:

- Property 3 in Proposition \ref{proposition-vector-product} says that
$$
(\uu \times \vv) \cdot \uu = 0 \,, \quad  (\uu \times \vv) \cdot \vv = 0 \,.
$$
Therefore $\uu \times \vv$ is orthogonal to both $\uu$ and $\vv$. 

- In particular $\uu \times \vv$ is orthogonal to the plane generated by $\uu$ and $\vv$.

- Since $\uu$ and $\vv$ are linearly independent, Property 2 in Proposition \ref{proposition-vector-product} says that
$$
\uu \times \vv \neq \zero
$$

- Therefore we have
$$
(\uu \times \vv) \cdot (\uu \times \vv) = \norm{ \uu \times \vv }^2 > 0 
$$

- On the other hand, using the definition of $\uu \times \vv$ with $\ww = \vv \times \ww$ yields
$$
(\uu \times \vv) \cdot (\uu \times \vv) =
\left|
\begin{array}{ccc}
u_1 & u_2 & u_3 \\
v_1 & v_2 & v_3 \\
(\uu \times \vv)_1 & (\uu \times \vv)_2 & (\uu \times \vv)_3 \\
\end{array}
\right| 
$$

- Therefore the determinant of the matrix
$$
(\uu | \vv | \uu \times \vv)
$$
is positive. This shows that 
$$
(\uu , \vv , \uu \times \vv)
$$
is a **positive basis** of $\R^3$.

- For all $\uu,\vv,\xx,\yy \in \R^3$ it holds
$$
(\uu \times \vv) \cdot (x \times y ) = 
\left|
\begin{array}{cc}
\uu \cdot \xx & \vv \cdot \xx  \\
\uu \cdot \yy & \vv \cdot \yy 
\end{array}
\right| \,.
$${#eq-formula-cross}
Indeed, one can check that the above formula holds for the standard vectors $\ee_i$, and thus the general formula follows by linearity.

- Using (@eq-formula-cross) we get
\begin{align}
\norm{\uu \times \vv}^2 & = (\uu \times \vv) \cdot (\uu \times \vv) = 
\left|
\begin{array}{cc}
\uu \cdot \uu & \vv \cdot \uu  \\
\uu \cdot \vv & \vv \cdot \vv 
\end{array}
\right|   \\
& = \norm{\uu}^2 \norm{\vv}^2 - |\uu \cdot \vv|^2 \\
& = \norm{\uu}^2 \norm{\vv}^2 - \norm{\uu}^2 \norm{\vv}^2 \cos^2(\theta) \\
& = \norm{\uu}^2\norm{\vv}^2 (1-\cos^2(\theta)) \\
& = \norm{\uu}^2\norm{\vv}^2 \sin^2(\theta) \\
& = A^2  
\end{align} 
where $A$ is the area of the parallelogram with sides $\uu$ and $\vv$.
:::


![For $\uu,\vv$ linearly independent, $\uu \times \vv$ is orthogonal to the plane generated by $\uu,\vv$. Moreover $|\uu \times \vv|$ is the area of the parallelogram with sides $\uu,\vv$, and $(\uu,\vv,\uu \times \vv)$ is a positive basis of $\R^3$](/images/vector_product_orthogonal.png){width=70%}


Let us summarize the above remark.

::: Remark
### Summary: Properties of $\uu \times \vv$

Let $\uu,\vv \in \R^3$ be linearly independent. Then

- $\uu \times \vv$ is orthogonal to the plane spanned by $\uu,\vv$
- $\norm{\uu \times \vv}$ is equal to the area of the parallelogram with sides $\uu,\vv$
- $\uu \times \vv$ is such that
$$
(\uu,\vv,\uu \times \vv)
$$
is a positive basis of $\R^3$.

:::



We conclude with a useful proposition for differentiating the cross product of curves in $\R^3$.


::: Proposition

Suppose $\g,\eeta \ \colon (a,b) \to \R^3$ are parametrized curves. Then
the curve 
$$
\g \times \eeta \ \colon (a,b) \to \R^3
$$
is smooth, and
$$
\frac{d}{dt} ( \g \times \eeta ) = \dot \g \times \eeta + \g \times \dot \eeta \,.
$$

:::

The proof is omitted. It follows immediately from formula (@eq-formula-cross-product).






## Curvature formula in $\R^3$


Given a unit speed curve
$$
\g \ \colon (a,b) \to \R^n
$$
we defined its curvature as
$$
\kappa(t) = \norm{ \ddot{\g}(t) } \,.
$$
If $\g$ is not unit speed then the curvature is not defined. However, when $\g$ is regular, then we can find a unit-speed reparametrization $\tg$ of $\g$, and compute $\kappa$ as
$$
\kappa(t) = \norm{ \ddot{\tg}(t) } \,.
$$
If $\g$ is a regular curve in $\R^3$, there is a way to compute $\kappa$ without passing through $\tg$. The formula for computing $\kappa$ is as follows. 

::: Proposition

Let $\g \colon (a,b) \to \R^3$ be a regular curve. Then the curvature $\kappa(t)$ of $\g$ at $\g(t)$ is given by
$$
\kappa(t) = \frac{ \norm{\dot \g \times \ddot \g} }{ \norm{\dot \g}^3 } \,. 
$${#eq-curvature}

:::


We delay the proof of the above Proposition, as this will get easier when the **Frenet frame** is introduced. For a proof which does not make use of the Frenet frame, see the proof of Proposition 2.1.2 in [@pressley].

For now we use (@eq-curvature) the above proposition to compute the curvature on specific curves.


::: Example

Consider the straight line
$$
\g(t) = \mathbf{a} + t \mathbf{v}
$$
for some $\mathbf{a}, \mathbf{v} \in \R^3$ fixed, with $\mathbf{v} \neq \zero$. Then
$$
\dot \g (t) = \mathbf{v} \,, \quad \ddot \g(t) = \zero \,. 
$$
Therefore 
$$
\norm{\dot \g (t)} = \norm{\mathbf{v}} \neq 0
$$
showing that $\g$ is regular. We have
$$
\dot \g \times \ddot \g = \mathbf{v} \times \zero = \zero \,.
$$
Therefore the curvature is
$$
\kappa = \frac{ \norm{ \dot \g \times \ddot \g } }{ \norm{\dot\g}^3 } = 0 \,,
$$
as expected.
:::



::: Example

Consider the Helix of radius $R>0$ and rise $H>0$
$$
\g (t) = ( R\cos(t) , R\sin(t) , Ht) \,, \quad t \in \R \,.
$$
Then
\begin{align}
\dot\g (t) & = ( -R\sin(t) , R\cos(t) , H)  \\
\ddot\g (t) & = ( -R\cos(t) , -R\sin(t) , 0) 
\end{align}
From this we deduce that
$$
\norm{\dot\g (t)}  = \sqrt{R^2 + H^2}\,,
$$
showing that $\g$ is regular. Finally
\begin{align}
\ddot \g \times \dot \g & = 
\left|
\begin{array}{cc}
{\dot\g}_2 & {\dot\g}_3  \\
{\ddot\g}_2 & {\ddot\g}_3
\end{array}
\right| \ee_1 -
\left|
\begin{array}{cc}
{\dot\g}_1 & {\dot\g}_3  \\
{\ddot\g}_1 & {\ddot\g}_3
\end{array}
\right| \ee_2 +
\left|
\begin{array}{cc}
{\dot\g}_1 & {\dot\g}_2  \\
{\ddot\g}_1 & {\ddot\g}_2
\end{array}
\right| \ee_3 \\
& = 
\left|
\begin{array}{cc}
R\cos(t) & H \\
-R\sin(t) & 0
\end{array}
\right| \ee_1 -
\left|
\begin{array}{cc}
-R\sin(t) & H \\
-R\cos(t) & 0 
\end{array}
\right| \ee_2 +
\left|
\begin{array}{cc}
-R\sin(t) & R\cos(t) \\
-R\cos(t) & -R\sin(t)  
\end{array}
\right| \ee_3 \\
& = 
\left(   
RH\sin(t),    
-RH\cos(t),
 R^2\cos^2(t) + R^2\sin^2(t)
\right) \\
& = 
\left(   
RH\sin(t),    
-RH\cos(t),
R^2
\right) 
\end{align}
and therefore
$$
\norm{ \dot \g \times \ddot \g } =  R\sqrt{R^2 + H^2   } \,.
$$
By the general formula we have
$$
\kappa = \frac{ \norm{ \dot \g \times \ddot \g } }{ \norm{\dot\g}^3 } =
\frac{ R (R^2 + H^2)^{\frac12} }{  (R^2 + H^2)^{\frac32}    } =
\frac{ R }{  R^2 + H^2   } 
$$

We notice the following:

- If $H=0$ then the Helix is just a circle of radius $R$. In this case the curvature is
$$
\kappa  = \frac{1}{R}
$$
which agrees with the curvature computed for the circle of radius $R$.

- If $R=0$ then the Helix is just parametrizing the $z$-axis. In this case the curvature is
$$
\kappa  = 0 \,,
$$
which agrees with the curvature of a straight line.

:::






## Signed curvature of plane curves

In this section we assume to have plane curves, that is, curves with values in $\R^2$. In this case we can give a geometric interpretation for the sign of the curvature. This cannot be done in higher dimension.


::: Definition

Let $\g \ \colon (a,b) \to \R^2$ be unit speed. We define the **signed unit normal** to $\g$ at $\g(t)$ as the unit vector $\nn(t)$ obtained by rotating $\dot \g(t)$ anti-clockwise by an angle of $\pi/2$.

:::


::: Definition

Let $\g \ \colon (a,b) \to \R^2$ be unit speed. The **signed curvature** of $\g$ at $\g(t)$ is the scalar $\kappa_s(t)$ such that
$$
\ddot \g(t) = k_s(t) \nn(t)
$$
:::

::: Remark
Notice that since $\nn$ is a unit vector and $\g$ is unit speed, then
$$
|\kappa_s(t)| = \norm{\ddot \g(t)} = \kappa(t) \,.
$$
Thus the signed curvature is related to the curvature by
$$
\kappa_s(t) = \pm \kappa(t) \,.
$$
:::


::: Remark
It can be shown that the signed curvature is the rate at which the tangent vector $\dot \g$ of the curve $\g$ rotates. The signed curvature is:

- positive if $\dot \g$ is rotating anti-clockwise
- negative if $\dot \g$ is rotating clockwise

In other words, 

- $k_s > 0$ means the curve is turning left,
- $k_s < 0$ means the curve is turning right.

A rigorous justification of the above statement is found in Proposition 2.2.3 in [@pressley].
:::



For curves which are not unit speed, we define the signed curvature as the signed curvature of the unit speed reparametrization. 



::: Definition

Let $\g \ \colon (a,b) \to \R^2$ be regular and let $\tg$ be a unit speed reparametrization of $\g$. The **signed curvature** of $\g$ at $\g(t)$ is the scalar $\kappa_s(t)$ such that
$$
\ddot{\tg}(t) = k_s(t) \nn(t) \,,
$$
where $\nn(t)$ is the unit vector obtained by rotating $\dot{\tg}(t)$ anti-clockwise by an angle $\pi/2$.
:::


The signed curvature completely characterizes plane curves, in the sense of the following theorem.


::: Theorem

Let $\f \ \colon \R \to \R$ be smooth. Then:

1. There exists a parametrized curve $\g \ \colon \R \to \R^2$ such that its signed curvature $\kappa_s$ satisfies
$$
\kappa_s(t) = \f(t) \,, \quad \forall \, t \in \R \,.
$$

2. Suppose that $\tg \ \colon \R \to \R^2$ is any curve such that its signed curvature $\tilde{\kappa}_s$ satisfies
$$
\tilde{\kappa}_s(t) = \f(t) \,, \quad \forall \, t \in \R \,.
$$
Then 
$$
\tg = \g
$$
up to rotations and translations.
:::


We do not prove the above theorem. For a proof, see Theorem 2.2.6 in [@pressley].






## Space curves

In this section we deal with **space curves**, that is, curves with values in $\R^3$. There are several issues compare to the plane case:

- A 3D counterpart of the signed curvature does not exist, since there is no notion of *turning left* or *turning right*.

- We have seen in the previous section that the signed curvature completely characterizes plane curves. In 3D however curvature is not enough to characterize curves: there exist $\g$ and $\eeta$ space curves such that 
$$
\kappa^{\g} = \kappa^{\eeta} \,, \quad  \g \neq \eeta \,,
$$
that is, $\g$ and $\eeta$ have same curvature but are different curves.



::: Example

Let $\g$ be a circle of radius $R>0$
$$
\g(t) = (R\cos(t),R\sin(t),0) \,,
$$
and $\eeta$ be a helix of radius $S>0$ and rise $H>0$
$$
\eeta(t) = (S\cos(t),S\sin(t),Ht) \,.
$$
We have computed that 
$$
\kappa^\g = \frac{1}{R}\,, \quad 
\kappa^\eeta = \frac{S}{\sqrt{S^2 + H^2}} \,.
$$


:::


